doc/book/code/Divergence.fst
@@ -181,7 +181,7 @@ let lift (op: int -> int -> int) (n m:dyn) : dyn
   = match n, m with
     | DInt i, DInt j -> DInt (op i j)
     | _ -> DErr "Expected integers"
-let mul = lift op_Multiply
+let mul = lift op_Star
 let sub = lift op_Subtraction
 let add = lift op_Addition
 let div (n m:dyn)
