examples/tactics/Arith.fst
@@ -22,7 +22,7 @@ open FStar.Tactics.Arith
 open FStar.List
 
 let lem0 (x:int) =
-    assert (op_Multiply 2 (x + 3) == 6 + (op_Multiply 3 x) - x)
+    assert (2 * (x + 3) == 6 + (3 * x) - x)
         by (prune ""; addns "Prims")
 
 // Can't locally define tactics
@@ -38,11 +38,11 @@ let tau1 () : Tac unit =
       smt ()
 
 let lem1 (x:int) =
-    assert (List.rev [1;2;3;4] == [4;3;2;1] /\ op_Multiply 2 (x + 3) == 6 + (op_Multiply 3 x) - x)
+    assert (List.rev [1;2;3;4] == [4;3;2;1] /\ 2 * (x + 3) == 6 + (3 * x) - x)
         by tau1 ()
 
 let lem2 (x:int) =
-    assert (List.rev [1;2;3;4] == [4;3;2;1] /\ op_Multiply 2 (x + 3) == 6 + (op_Multiply 3 x) - x)
+    assert (List.rev [1;2;3;4] == [4;3;2;1] /\ 2 * (x + 3) == 6 + (3 * x) - x)
         by split_arith ()
 
 let lem3 (x y z : int) (f : int -> int) =
@@ -54,5 +54,5 @@ let lem4 (x y z : int) (f : int -> int) =
     assume (forall y. f y > y);
     assert (f 5 > 1 /\ f == f /\ List.length (List.Tot.tail [1;2;3]) == 2
             /\ 1 + 2 == 3 /\ (forall x. f (f x) > x)
-            /\ (forall (x y : int). x > 2 /\ y > 2 ==> op_Multiply x y > x + y))
+            /\ (forall (x y : int). x > 2 /\ y > 2 ==> x * y > x + y))
         by split_arith ()
