src/smtencoding/FStarC.SMTEncoding.EncodeTerm.fst
@@ -295,7 +295,7 @@ let is_arithmetic_primitive head args =
     | Tm_fvar fv, [_;_]->
       S.fv_eq_lid fv Const.op_Addition
       || S.fv_eq_lid fv Const.op_Subtraction
-      || S.fv_eq_lid fv Const.op_Multiply
+      || S.fv_eq_lid fv Const.op_Star
       || S.fv_eq_lid fv Const.op_Division
       || S.fv_eq_lid fv Const.op_Modulus
       || S.fv_eq_lid fv Const.real_op_LT
@@ -475,7 +475,7 @@ and encode_arith_term env head args_e : ML _ =
     let ops : list (Ident.lident & (list term -> ML term)) =
         [(Const.op_Addition,    add Term.boxInt Term.unboxInt);
          (Const.op_Subtraction, sub Term.boxInt Term.unboxInt);
-         (Const.op_Multiply,    mul Term.boxInt Term.unboxInt "_mul");
+         (Const.op_Star,        mul Term.boxInt Term.unboxInt "_mul");
          (Const.op_Division,    div Term.boxInt Term.unboxInt "_div");
          (Const.op_Modulus,     modulus Term.boxInt Term.unboxInt);
          (Const.op_Minus,       minus Term.boxInt Term.unboxInt);
