ulib/FStar.Tactics.Canon.fst
@@ -41,7 +41,7 @@ let rec canon_point e =
         Lit (a + b)
 
     | Mult (Lit a) (Lit b) ->
-        norm [delta; primops]; // Need delta to turn op_Star into op_Multiply, as there's no primop for it
+        norm [primops];
         trefl ();
         Lit (a * b)
 
